finished the tables properties

hol/tables_specScript.sml
@@ -171,7 +171,15 @@ Definition sem_tables_def:
 End
 
 
+(*
+EVAL “match_tbl [([False], 0 , action "s")] [] 0”
+EVAL “match_tbl [([True], 0 , action "s")] [] 0”
+EVAL “match_tbl [([Var "a"], 0 , action "s1");([True], 0 , action "s2")] [("a",T)] 0”
 
+EVAL “final_tbl [([Var "a"], 0 , action "s1");([True], 0 , action "s2")] 0”
+
+     
+*)
 
       
 (* table substitute *)
@@ -230,6 +238,12 @@ Definition all_true_def:
   EVERY (\atom. atom = True) atoml
 End
 
+
+Definition all_false_def:
+  all_false atoml =
+  EVERY (\atom. atom = False) atoml
+End
+        
        
 Definition is_hit_def:
   is_hit st_in st_num atoml = 
@@ -246,7 +260,7 @@ End
 
 Definition pre_lines_are_fail_def:
   pre_lines_are_fail (tbl: 'a table) idx =
-  EVERY (\(atoml, st_num, res). ~ all_true atoml) (SEG idx 0 tbl)
+  EVERY (\(atoml, st_num, res).  all_false atoml) (SEG idx 0 tbl)
 End
 
         
@@ -261,7 +275,15 @@ Definition final_tbl_def:
         )
     | _ => NONE
 End
- 
+
+(*
+EVAL “final_tbl [([False], 0 , action "s")] 0”
+EVAL “final_tbl [([True], 0 , action "s")] 0”
+EVAL “final_tbl [([False], 0 , action "s1");([True], 0 , action "s2")] 0”
+EVAL “final_tbl [([Var "a"], 0 , action "s1");([True], 0 , action "s2")] 0”
+
+*)
+        
         
 Definition final_tbll_def:
   final_tbll ([]: 'a table_list) st_in = NONE ∧
@@ -872,8 +894,673 @@ Proof
 QED
 
 
+Theorem is_hit_true_atoml_not_empty:
+  ∀ atoml h' b s_in st_num.        
+    is_hit s_in st_num (simp_row (mk_substitute_row atoml h' b)) ⇒
+    atoml ≠ []
+Proof
+  gvs[is_hit_def, all_true_def, mk_substitute_row_def, simp_row_def]
+QED
+
+
+Theorem subst_simp_sound_for_atom:
+  ∀atom h' b mv.
+    ALOOKUP mv h' = SOME b ⇒
+    (simp_atom (mk_substitute_atom atom h' b) = True ⇒
+     sem_atom atom mv = SOME T) ∧
+    (simp_atom (mk_substitute_atom atom h' b) = False ⇒
+     sem_atom atom mv = SOME F)
+Proof                                   
+  Induct >-
+   gvs[simp_atom_def, mk_substitute_atom_def, sem_atom_def] >-
+   gvs[simp_atom_def, mk_substitute_atom_def, sem_atom_def] >>
+  gvs[simp_atom_def, mk_substitute_atom_def, sem_atom_def] >>
+  rpt strip_tac >>
+  rpt (BasicProvers.FULL_CASE_TAC >> gvs[simp_atom_def, mk_substitute_atom_def, sem_atom_def]) >>
+  res_tac >>
+  gvs[sem_atom_def]    
+QED
+
+
+                         
+Theorem hit_implies_match_after_subst:
+  ∀ atoml s_in st_num h' b mv.
+    ALOOKUP mv h' = SOME b ∧
+    is_hit s_in st_num (simp_row (mk_substitute_row atoml h' b)) ⇒
+    is_match_row s_in st_num atoml mv
+Proof
+  Induct_on ‘atoml’ >>
+  rpt strip_tac >>
+  imp_res_tac is_hit_true_atoml_not_empty >>               
+  gvs[is_hit_def, is_match_row_def] >>
+  gvs[is_atoml_true_def, mk_substitute_row_def, simp_row_def, all_true_def] >>
+  res_tac >>
+  Cases_on ‘atoml=[]’ >> gvs[] >>
+  imp_res_tac subst_simp_sound_for_atom      
+QED
+
+
         
-           
+        
+Theorem row_miss_preserved_by_subst_simp:
+  ∀ tbl s_in h' b mv.
+    ALOOKUP mv h' = SOME b ∧
+    EVERY ($¬ ∘ (λ(p,a). p)) (MAP (λ(atoml,st_num,res). (is_match_row s_in st_num atoml mv,res)) tbl)
+    ⇒
+    ¬ EXISTS (λx. (λ(p,a). p) ((λ(atoml,st_num,res). (is_hit s_in st_num atoml,st_num,res))
+                               ((λ(atoml,st_num,res). (simp_row atoml,st_num,res))
+                                ((λ(atoml,st_num,res). (mk_substitute_row atoml h' b,st_num,res)) x)))) tbl
+Proof
+Induct >> gvs[] >>                  
+rpt strip_tac >>
+PairCases_on ‘h’ >> gvs[] >>
+imp_res_tac hit_implies_match_after_subst >>
+res_tac
+QED
+
+
+
+Theorem pre_lines_are_fail_normalize:
+  ∀ l h idx.
+    idx > 0 ∧
+    idx < LENGTH (h::l) ∧
+    pre_lines_are_fail (h::l) idx ⇒
+    pre_lines_are_fail l (idx-1)
+Proof
+  rpt strip_tac >>
+  gvs[pre_lines_are_fail_def] >>
+  imp_res_tac every_seg_property_1 >>
+  Cases_on ‘idx’ >> gvs[SUC_ADD_ONE] >>
+  res_tac >>
+  imp_res_tac every_seg_property_1 >>
+  ‘n < LENGTH l’ by gvs[] >>
+  gvs[]
+QED
+
+
+
+       
+Theorem index_find_not_prev:
+  ∀ l P r.         
+    INDEX_FIND 1 P l ≠ SOME (0,r)            
+Proof
+  Induct >> gvs[INDEX_FIND_def] >>
+  rpt strip_tac >>
+  rpt (BasicProvers.FULL_CASE_TAC >> gvs[]) >>
+  assume_tac P_hold_on_next >>
+  first_x_assum (strip_assume_tac o (Q.SPECL [‘(1:num)’, ‘l’, ‘P’, ‘(0,r)’])) >>
+  gvs[SUC_ADD_ONE]
+QED
+                          
+        
+
+Theorem index_find_not_prev_gen:
+  ∀ i l P r .
+    i > 1 ∧
+    0 < LENGTH l ⇒
+    INDEX_FIND i P l ≠ SOME (i-1,r)
+Proof
+  Induct >> gvs[INDEX_FIND_def] >>
+  rpt strip_tac >>
+  rpt (BasicProvers.FULL_CASE_TAC >> gvs[]) >>
+  assume_tac P_hold_on_next >> 
+  first_x_assum (strip_assume_tac o (Q.SPECL [‘(i:num)’, ‘l’, ‘P’, ‘(i,r)’])) >>
+  gvs[SUC_ADD_ONE] >>
+
+  Cases_on ‘i > 1’ >> gvs[] >>
+  Cases_on ‘i=1’ >> gvs[] >>
+  imp_res_tac index_find_not_prev      
+QED
+
+
+
+
+
+Theorem every_seg_property_3:         
+  ∀ n l h p.
+    0 < n ∧
+    EVERY p (SEG n 0 (h::l)) ⇒
+    EVERY p (SEG (n-1) 0 l)
+Proof
+  Induct >>
+  rpt strip_tac >>
+  gvs[SEG, SUC_ADD_ONE] >>
+  gvs[GSYM TAKE_SEG]
+QED
+        
+                        
+        
+Theorem every_simp_false_imp_sem_false:
+  ∀ atoml h' b mv.
+    atoml ≠ [] ∧
+    ALOOKUP mv h' = SOME b ∧
+    EVERY (λatom. atom = False) (simp_row (mk_substitute_row atoml h' b)) ⇒
+    ~ EVERY (λminipred. sem_atom minipred mv = SOME T) atoml
+Proof
+  Induct >-
+   gvs[mk_substitute_row_def, simp_row_def] >>
+  rpt strip_tac >>
+  
+  gvs[all_true_def, simp_row_def, mk_substitute_row_def] >>
+  
+  imp_res_tac subst_simp_sound_for_atom >>
+  gvs[]
+QED
+
+
+Theorem subst_simp_miss_implies_sem_miss:
+  ∀ atoml h' b mv st_num s_in. 
+    ALOOKUP mv h' = SOME b ∧
+    ¬is_hit s_in st_num (simp_row (mk_substitute_row atoml h' b)) ∧
+    all_false (simp_row (mk_substitute_row atoml h' b)) ⇒
+    ¬is_match_row s_in st_num atoml mv
+Proof
+  rpt strip_tac >>                   
+  gvs[all_false_def, is_match_row_def, is_hit_def] >>
+  gvs[is_atoml_true_def] >-
+   imp_res_tac every_simp_false_imp_sem_false >>
+  gvs[mk_substitute_row_def, simp_row_def]
+QED
+
+
+
+
+        
+Theorem index_find_agreement_under_subst_and_all_false_prefix:       
+∀ tbl (s_in:num) n st_num res q (res':'a action_expr) h' b mv.
+  ALOOKUP mv h' = SOME b ∧
+EVERY (λ(atoml,st_num,res). all_false atoml)
+          (SEG n 0
+             (MAP
+                ((λ(atoml,st_num,res). (simp_row atoml,st_num,res)) ∘
+                 (λ(atoml,st_num,res).
+                      (mk_substitute_row atoml h' b,st_num,res))) tbl)) ∧
+INDEX_FIND 0 (λ(p,a). p)
+          (MAP (λ(atoml,st_num,res). (is_match_row s_in st_num atoml mv,res))
+             tbl) =
+        SOME (q − 1,T,res') ∧
+INDEX_FIND 0 (λ(p,a). p)
+          (MAP
+             ((λ(atoml,st_num,res). (is_hit s_in st_num atoml,st_num,res)) ∘
+              (λ(atoml,st_num,res). (simp_row atoml,st_num,res)) ∘
+              (λ(atoml,st_num,res). (mk_substitute_row atoml h' b,st_num,res)))
+             tbl) =
+        SOME (n,T,st_num,res) ⇒
+res=res'
+Proof
+
+Induct >|[
+    gvs[INDEX_FIND_def]
+    ,
+    rpt strip_tac >>
+    PairCases_on ‘h’ >>
+    gvs[INDEX_FIND_def] >>
+    rpt (BasicProvers.FULL_CASE_TAC >> gvs[]) >|[
+                                    
+        imp_res_tac hit_implies_match_after_subst
+        ,
+                
+        Cases_on ‘q=0’ >> gvs[] >|[
+          Cases_on ‘n’ >>
+          gvs[SEG, SUC_ADD_ONE] >>
+          gvs[GSYM TAKE_SEG] >>
+          gvs[index_find_not_prev] >>
+          imp_res_tac subst_simp_miss_implies_sem_miss
+          ,
+          ‘q=1’ by gvs[] >>
+          gvs[] >>
+           Cases_on ‘n’ >>
+          gvs[SEG, SUC_ADD_ONE] >>
+          gvs[GSYM TAKE_SEG] >>
+          gvs[index_find_not_prev] >>
+          imp_res_tac subst_simp_miss_implies_sem_miss
+          ]
+                                        
+        ,
+        
+        
+        assume_tac (INST_TYPE [“:'a” |-> “:(bool # 'a action_expr)”,
+                               “:'b” |-> “:num”] P_hold_on_next)  >>
+        first_x_assum (strip_assume_tac o (Q.SPECL [‘0’,
+         ‘(MAP (λ(atoml,st_num,res). (is_match_row (s_in:num) st_num atoml mv,res)) tbl)’,
+         ‘(λ(p,a). p)’, ‘(q − 1,T,(res':α action_expr))’])) >>
+        gvs[] >>
+
+
+
+
+        
+        assume_tac (INST_TYPE [“:'a” |-> “:(bool # num # 'a action_expr)”] P_hold_on_next)  >>
+        first_x_assum (strip_assume_tac o (Q.SPECL [‘0’,
+         ‘(MAP ((λ(atoml,st_num,res). (is_hit s_in st_num atoml,st_num,res)) ∘
+                (λ(atoml,st_num,res). (simp_row atoml,st_num,res)) ∘
+                (λ(atoml,st_num,res). (mk_substitute_row atoml h' b,st_num,res))) tbl)’,
+         ‘(λ(p,a). p)’, ‘(n,T,st_num,res)’])) >>
+        gvs[] >>
+
+
+
+        imp_res_tac every_seg_property_3 >>
+        last_x_assum (strip_assume_tac o (Q.SPECL [‘s_in’, ‘n-1’, ‘st_num’, ‘res’,
+                                                   ‘q-1’ ,‘res'’, ‘h'’, ‘b’, ‘mv’])) >>
+        gvs[]    
+      ]
+]
+QED
+
+
+
+
+                           
+    
+
+    
+Theorem prop2_var_single_tbl_verbose:
+  ∀ tbl mv h' b res s_in.
+    ALOOKUP mv h' = SOME b ∧
+    final_tbl (simp_tbl (mk_substitute_tbl tbl h' b)) s_in = SOME res ⇒
+    match_tbl tbl mv s_in = SOME res
+Proof       
+  
+  Cases_on ‘tbl’ >| [
+    gvs[fv_tbl_def, mk_substitute_tbl_def, simp_tbl_def, final_tbl_def,
+        min_idx_till_def, is_hit_tbl_check_def, INDEX_FIND_def]
+    ,
+    rpt strip_tac >>
+    gvs[mk_substitute_tbl_def, simp_tbl_def, final_tbl_def] >>
+    gvs[match_tbl_def] >>
+    rpt (BasicProvers.FULL_CASE_TAC >> gvs[]) >>
+    
+    rename1 ‘(idx,bool,st_num,res)’ >>
+    PairCases_on ‘h’ >>
+    gvs[is_hit_tbl_check_def, check_all_rows_match_def] >>
+    gvs[min_idx_till_def] >|[
+        gvs[INDEX_FIND_def] >>
+        rpt (BasicProvers.FULL_CASE_TAC >> gvs[])  >|[
+          imp_res_tac hit_implies_match_after_subst
+          ,
+          imp_res_tac INDEX_FIND_NONE_EXISTS >>
+          imp_res_tac exists_index_some >>
+          gvs[EXISTS_MAP] >>
+          gvs[MAP_MAP_o] >>
+          imp_res_tac row_miss_preserved_by_subst_simp
+        ]
+        ,
+
+
+        gvs[INDEX_FIND_def] >>
+        rpt (BasicProvers.FULL_CASE_TAC >> gvs[]) >|[
+          imp_res_tac hit_implies_match_after_subst
+          ,
+          gvs[pre_lines_are_fail_def] >>
+          Cases_on ‘idx’ >>
+          gvs[SEG, SUC_ADD_ONE] >>
+          gvs[GSYM TAKE_SEG] >>
+          gvs[index_find_not_prev] >>
+          imp_res_tac subst_simp_miss_implies_sem_miss
+          ,
+          
+          gvs[pre_lines_are_fail_def] >>
+          Cases_on ‘idx’ >>
+          gvs[SEG, SUC_ADD_ONE] >>
+          gvs[GSYM TAKE_SEG] >>
+          gvs[index_find_not_prev] >>
+          PairCases_on ‘r’ >> gvs[] >>
+
+          assume_tac (INST_TYPE [“:'a” |-> “:(bool # 'a action_expr)”,
+                                 “:'b” |-> “:num”] P_hold_on_next)  >>
+          first_x_assum (strip_assume_tac o (Q.SPECL [‘0’,
+            ‘(MAP (λ(atoml,st_num,res). (is_match_row (s_in:num) st_num atoml mv,res)) t)’,
+            ‘(λ(p,a). p)’, ‘(q,r0,r1)’])) >>
+          gvs[] >>
+
+          assume_tac (INST_TYPE [“:'a” |-> “:(bool # num # 'a action_expr)”] P_hold_on_next)  >>
+          first_x_assum (strip_assume_tac o (Q.SPECL [‘0’,
+            ‘(MAP (λ(atoml,st_num,res). (is_hit s_in st_num atoml,st_num,res))
+             (MAP (λ(atoml,st_num,res). (simp_row atoml,st_num,res))
+             (MAP (λ(atoml,st_num,res). (mk_substitute_row atoml h' b,st_num,res)) t)))’,
+            ‘(λ(p,a). p)’, ‘(n + 1,bool,st_num,res)’])) >>
+
+
+          gvs[] >>
+          
+          
+          ‘(λ(p,a). p) (bool,st_num,res)’ by imp_res_tac INDEX_FIND_EQ_SOME_0 >>
+          ‘(λ(p,a). p) (r0,r1)’ by imp_res_tac INDEX_FIND_EQ_SOME_0 >>
+          
+          gvs[] >>
+        
+          
+          gvs[MAP_MAP_o] >>
+          imp_res_tac index_find_agreement_under_subst_and_all_false_prefix >>
+          gvs[]
+          ] 
+      ]
+  ]
+QED
+
+
+        
+
+Theorem prop2_var_tables_verbose:
+  ∀ tbls h b mv s_in res.
+    ALOOKUP mv h = SOME b ∧
+    final_tbll (simp_tbll (mk_substitute_tbll tbls h b)) s_in = SOME res ⇒
+    sem_tables (tbls,s_in) mv = SOME res 
+Proof
+
+  Induct_on ‘tbls’ >> rpt strip_tac >-
+   gvs[mk_substitute_tbll_def, simp_tbll_def, final_tbll_def] >> 
+  rename1 ‘(tbl::tbll)’ >>
+
+
+  Cases_on ‘tbll’ >> gvs[] >|[
+    
+    gvs[sem_tables_def, match_tbll_def] >>
+    gvs[mk_substitute_tbll_def, simp_tbll_def, final_tbll_def] >>
+    gvs[] >>
+    rpt (BasicProvers.FULL_CASE_TAC >> gvs[]) >>
+    
+    imp_res_tac prop2_var_single_tbl_verbose >> gvs[]              
+    ,
+    rename1 ‘(tbl::nexttbl::tbll)’ >>
+    rgs[Once mk_substitute_tbll_def, Once simp_tbll_def] >>
+    rgs[Once final_tbll_def] >>     
+
+    Cases_on ‘final_tbl (simp_tbl (mk_substitute_tbl tbl h' b)) s_in’ >>
+    gvs[] >>
+    Cases_on ‘x’ >>
+    gvs[] >>
+    
+    rgs[Once mk_substitute_tbll_def, Once simp_tbll_def] >>
+    rgs[Once final_tbll_def] >>  
+    res_tac >>
+
+    gvs[sem_tables_def, match_tbll_def] >>
+    gvs[mk_substitute_tbll_def, simp_tbll_def, final_tbll_def] >>
+    gvs[] >>
+    rpt (BasicProvers.FULL_CASE_TAC >> gvs[]) >>
+    
+    imp_res_tac prop2_var_single_tbl_verbose >> gvs[]     
+  ]
+QED
+
+
+
+Theorem prop2_var_tables:
+  prop2 table_structure
+Proof
+  rgs[prop2_def, table_structure_def, fv_in_p_def] >>
+
+  rpt strip_tac >>
+  Cases_on ‘p’ >>
+  rename1 ‘(tbls, s_in)’ >>
+
+  gvs[final_tables_def, fv_tables_def, mk_substitute_tables_def, simp_tables_def] >>
+  imp_res_tac prop1_var_tables_verbose >> gvs[] >>
+  imp_res_tac prop2_var_tables_verbose >> gvs[]
+QED
+
+
+                   
+Theorem hit_implies_match_after_all:
+  ∀ atoml s_in st_num h' b mv.
+    is_hit s_in st_num atoml ⇒
+    is_match_row s_in st_num atoml mv
+Proof
+  Induct_on ‘atoml’ >>
+  rpt strip_tac >>
+  gvs[is_hit_def, is_match_row_def] >>
+  gvs[is_atoml_true_def,all_true_def] >>
+  res_tac >>
+  Cases_on ‘atoml=[]’ >>
+  gvs[sem_atom_def]
+QED
+
+
+
+Theorem subst_simp_miss_implies_sem_miss_full:
+  ∀ atoml h' b mv s_in st_num .
+    ¬is_hit s_in st_num (simp_row (mk_substitute_row atoml h' b)) ∧
+    all_false (simp_row (mk_substitute_row atoml h' b)) ⇒
+    ¬is_match_row s_in st_num  (simp_row (mk_substitute_row atoml h' b)) mv
+Proof
+  Induct >>
+  rpt strip_tac >>                   
+  gvs[all_false_def, is_match_row_def, is_hit_def] >>
+  gvs[is_atoml_true_def, all_true_def] >>
+  gvs[mk_substitute_row_def, simp_row_def] >>
+  res_tac >>
+  gvs[mk_substitute_row_def, simp_row_def, sem_atom_def]
+QED
+
+
+
+        
+
+Theorem match_follows_hit_at_minimal_index:
+  ∀ tbl s_in idx  bool  st_num res mv h' b.
+    pre_lines_are_fail (simp_tbl (mk_substitute_tbl tbl h' b)) idx ∧
+    min_idx_till (is_hit_tbl_check (simp_tbl (mk_substitute_tbl tbl h' b)) s_in) T =
+    SOME (idx,bool,st_num,res)  ⇒
+    min_idx_till (check_all_rows_match s_in (simp_tbl (mk_substitute_tbl tbl h' b)) mv) T =
+    SOME (idx,bool,res)
+Proof
+gvs[min_idx_till_def] >>
+Induct >>
+rpt strip_tac >-
+ gvs[mk_substitute_tbl_def, check_all_rows_match_def, simp_tbl_def,
+     is_hit_tbl_check_def, INDEX_FIND_def] >>
+
+
+  PairCases_on ‘h’ >>
+  gvs[simp_tbl_def, mk_substitute_tbl_def, is_hit_tbl_check_def] >>
+gvs[INDEX_FIND_def]>>
+rpt (BasicProvers.FULL_CASE_TAC >> gvs[]) >|[
+    
+    gvs[check_all_rows_match_def, INDEX_FIND_def] >>
+    rpt (BasicProvers.FULL_CASE_TAC >> gvs[])>>
+    imp_res_tac hit_implies_match_after_all >>
+    gvs[]
+    ,
+
+    gvs[check_all_rows_match_def, INDEX_FIND_def]>>
+    rpt (BasicProvers.FULL_CASE_TAC >> gvs[]) >|[
+        Cases_on ‘bool’ >>
+        gvs[pre_lines_are_fail_def] >>
+         Cases_on ‘idx’ >>
+          gvs[SEG, SUC_ADD_ONE] >>
+          gvs[GSYM TAKE_SEG] >>
+          gvs[index_find_not_prev] >>
+        imp_res_tac subst_simp_miss_implies_sem_miss_full
+        ,
+        gvs[MAP_MAP_o] >>
+        gvs[pre_lines_are_fail_def] >>
+        Cases_on ‘idx’ >>
+        gvs[SEG, SUC_ADD_ONE] >>
+        gvs[GSYM TAKE_SEG] >>
+        gvs[index_find_not_prev] >>
+        
+        
+        
+        assume_tac (INST_TYPE [“:'a” |-> “:(bool # num # 'a action_expr)”] P_hold_on_next)  >>
+        first_x_assum (strip_assume_tac o (Q.SPECL [‘0’,
+            ‘(MAP ((λ(atoml,st_num,res). (is_hit s_in st_num atoml,st_num,res)) ∘
+              (λ(atoml,st_num,res). (simp_row atoml,st_num,res)) ∘
+              (λ(atoml,st_num,res). (mk_substitute_row atoml h' b,st_num,res))) tbl)’,
+            ‘(λ(p,a). p)’, ‘(n + 1,bool,st_num,res)’])) >>
+          gvs[] >>
+          
+        
+        res_tac >>
+        first_x_assum (strip_assume_tac o (Q.SPECL [‘mv’])) >>
+        drule P_implies_next >>
+        gvs[]
+  ] 
+]
+QED
+
+
+
+Theorem final_tbl_yields_match_tbl:      
+  ∀ tbl s_in mv res h' b.
+    final_tbl (simp_tbl (mk_substitute_tbl tbl h' b)) s_in = SOME res ⇒
+    match_tbl (simp_tbl (mk_substitute_tbl tbl h' b)) mv s_in = SOME res
+Proof
+  rpt strip_tac >>
+  gvs[final_tbl_def, match_tbl_def] >>
+  rpt (BasicProvers.FULL_CASE_TAC >> gvs[]) >>
+  imp_res_tac match_follows_hit_at_minimal_index >> gvs[]
+QED
+
+
+Theorem final_tbll_yields_match_tbll:                            
+  ∀ tbll s_in h b mv q .
+    final_tbll (simp_tbll (mk_substitute_tbll tbll h b)) s_in = SOME q ⇒
+    match_tbll (simp_tbll (mk_substitute_tbll tbll h b))  mv s_in = SOME q
+Proof
+
+Induct >-
+(gvs[mk_substitute_tbll_def, simp_tbll_def, final_tbll_def]) >>
+
+                     
+rpt strip_tac >>
+Cases_on ‘tbll’ >|[
+simp[match_tbll_def] >>
+gvs[mk_substitute_tbll_def, simp_tbll_def, final_tbll_def] >>
+rpt (BasicProvers.FULL_CASE_TAC >> gvs[]) >>
+imp_res_tac final_tbl_yields_match_tbl >> gvs[match_tbll_def]
+,
+
+gvs[mk_substitute_tbll_def, simp_tbll_def, final_tbll_def] >>
+rpt (BasicProvers.FULL_CASE_TAC >> gvs[]) >>
+res_tac >>
+
+gvs[match_tbll_def] >>
+rpt (BasicProvers.FULL_CASE_TAC >> gvs[]) >>
+imp_res_tac final_tbl_yields_match_tbl >> gvs[match_tbll_def]
+]
+QED
+
+
+
+
+Theorem prop3_var_tables:
+  prop3 table_structure
+Proof
+  rgs[prop3_def, table_structure_def, fv_in_p_def] >>
+
+  rpt strip_tac >>
+  Cases_on ‘p’ >>
+  rename1 ‘(tbls, s_in)’ >>
+  gvs[final_tables_def, simp_tables_def, mk_substitute_tables_def, sem_tables_def] >>
+  imp_res_tac final_tbll_yields_match_tbll >> gvs[]
+QED
+
+
+
+
+
+
+Theorem fv_mem_tbll_varslist_thm:
+  ∀ tbll tbl varslist.
+    (∀x. MEM x (fv_tbll (tbl::tbll)) ⇒ MEM x varslist) ⇒
+    (∀x. MEM x (fv_tbll  tbll) ⇒  MEM x varslist)
+Proof
+  gvs[fv_tbll_def]
+QED
+
+
+
+Theorem free_vars_simp_subst_in_original:
+  ∀ atom h' b x.
+    MEM x (fv_atom (simp_atom (mk_substitute_atom atom h' b))) ⇒
+    MEM x (fv_atom atom)
+Proof
+  Induct >>
+  gvs[fv_atom_def, simp_atom_def, mk_substitute_atom_def] >>
+  rpt strip_tac >>
+  rpt (BasicProvers.FULL_CASE_TAC >> gvs[]) >>
+  gvs[fv_atom_def, simp_atom_def, mk_substitute_atom_def] >>
+  imp_res_tac sub_then_simp_answer_indeed_in_fv >>
+  res_tac >>
+  imp_res_tac simp_fv_not_triv1 >>
+  res_tac 
+QED
+      
+
+        
+Theorem free_vars_simp_subst_row_in_original:
+  ∀ row h' b x.
+    MEM x (fv_row (simp_row (mk_substitute_row row h' b))) ⇒
+    MEM x (fv_row row)
+Proof
+  Induct >>
+  gvs[fv_row_def, simp_row_def, mk_substitute_row_def] >>
+  rpt strip_tac >|[
+    imp_res_tac free_vars_simp_subst_in_original >> gvs[]
+    ,
+    res_tac >> gvs[]
+  ]
+QED
+
+      
+Theorem free_vars_simp_subst_tbl_in_original:
+  ∀ tbl x h' b.
+    MEM x (fv_tbl (simp_tbl (mk_substitute_tbl tbl h' b))) ⇒
+    MEM x (fv_tbl tbl)
+Proof
+  Induct >>
+  rpt strip_tac >>
+  gvs[fv_tbl_def, mk_substitute_tbl_def, simp_tbl_def] >|[
+    PairCases_on ‘h’ >> gvs[] >>
+    imp_res_tac free_vars_simp_subst_row_in_original >>
+    gvs[]
+    ,
+    res_tac >> gvs[]
+  ]
+QED                                                         
+      
+
+Theorem free_vars_simp_subst_tbll_in_original:
+  ∀ tbls h b x varslist.
+    (∀x'. MEM x' (fv_tbll tbls) ⇒ MEM x' varslist) ∧
+    MEM x (fv_tbll (simp_tbll (mk_substitute_tbll tbls h b))) ⇒
+    MEM x varslist
+Proof
+  Induct >-
+   (gvs[fv_tbll_def, mk_substitute_tbll_def, simp_tbll_def]) >>
+  
+  rpt strip_tac >>    
+  gvs[mk_substitute_tbll_def, simp_tbll_def] >>
+  imp_res_tac fv_mem_tbll_varslist_thm >>
+  res_tac >>
+  gvs[fv_tbll_def] >|[
+    imp_res_tac free_vars_simp_subst_tbl_in_original >>
+    gvs[]
+    ,
+    metis_tac[]      
+  ]                            
+QED
+
+        
+
+Theorem prop4_var_tables:
+  prop4 table_structure
+Proof
+  rgs[prop4_def, table_structure_def, fv_in_p_def, fv_in_vars_def] >>
+
+  rpt strip_tac >>
+  Cases_on ‘prop_parent’ >>
+  rename1 ‘(tbls, s_in)’ >>
+  gvs[fv_tables_def, simp_tables_def, mk_substitute_tables_def] >>
+  imp_res_tac free_vars_simp_subst_tbll_in_original
+QED
+
+
+
+
+                 
 val _ = export_theory ();
 
     
